Prove join is the inversion function of split in Memory

specs/Memory.v
@@ -2,6 +2,7 @@ Require Import Coq.Arith.Arith.
 Require Import Coq.Program.Program.
 Require Import Coq.Setoids.Setoid.
 Require Import Omega.
+Require Import FreeSpec.Control.
 
 Require Import FreeSpec.Libs.OpenNat.OpenNat.
 Require Import FreeSpec.PropBool.
@@ -29,17 +30,19 @@ Definition qword := mem 64.
 Notation "x 'Byte'" := (x * 8) (at level 30, no associativity).
 Notation "x 'Bytes'" := (x * 8) (at level 30, no associativity).
 
-Definition mem_eq
-           {n: nat}
-           (m m': mem n)
+Inductive mem_eq
+          {n:     nat}
+          (m m':  mem n)
   : Prop :=
-  mem_val m = mem_val m'.
+| mem_val_eq (H:  mem_val m = mem_val m')
+  : mem_eq m m'.
 
 Lemma mem_eq_refl
       {n: nat}
       (m: mem n)
   : mem_eq m m.
 Proof.
+  constructor.
   reflexivity.
 Qed.
 
@@ -48,7 +51,8 @@ Lemma mem_eq_sym
       (m m': mem n)
   : mem_eq m m' -> mem_eq m' m.
 Proof.
-  intros.
+  intros [H].
+  constructor.
   symmetry.
   exact H.
 Qed.
@@ -60,7 +64,8 @@ Lemma mem_eq_trans
     -> mem_eq m' m''
     -> mem_eq m m''.
 Proof.
-  intros H H'.
+  intros [H] [H'].
+  constructor.
   transitivity (mem_val m').
   + exact H.
   + exact H'.
@@ -86,6 +91,16 @@ Definition mem_bool
   : bool :=
   Nat.eqb (mem_val m) (mem_val m').
 
+Add Parametric Morphism
+    (n:  nat)
+  : mem_bool with signature (@mem_eq n) ==> (@mem_eq n) ==> eq
+      as mem_bool_morphism.
+  intros x x' [Heq] y y' [Heq'].
+  unfold mem_bool.
+  rewrite Heq; rewrite Heq'.
+  reflexivity.
+Qed.
+
 Instance mem_bool_propbool
          (n:  nat)
   : PropBool2 (@mem_eq n) (@mem_bool n) :=
@@ -93,8 +108,16 @@ Instance mem_bool_propbool
   }.
 Proof.
   intros m m'.
-  unfold mem_eq, mem_bool.
-  apply (Nat.eqb_eq (mem_val m) (mem_val m')).
+  split.
+  + intro H.
+    constructor.
+    unfold mem_bool in H.
+    apply (Nat.eqb_eq (mem_val m) (mem_val m')).
+    exact H.
+  + intros [H].
+    unfold mem_bool.
+    apply (Nat.eqb_eq (mem_val m) (mem_val m')).
+    exact H.
 Defined.
 
 Instance mem_WEqBool
@@ -111,41 +134,14 @@ Instance mem_WEqBool
 Program Definition box
         (n x: nat)
   : mem n :=
-  {| mem_val := if lt_dec x (2 ^ n)
-                then x
-                else x mod (2 ^ n)
+  {| mem_val := x mod (2 ^ n)
    ; mem_bound := _
    |}.
 Next Obligation.
-  destruct (lt_dec  x (2 ^ n)).
-  + exact l.
-  + apply Nat.mod_bound_pos.
-    ++ apply OpenNat.le_0_n.
-    ++ assert (G: forall z, 0 < 2 ^ z). {
-         clear x n0.
-         induction z.
-         + constructor.
-         + cbn.
-           rewrite OpenNat.add_0_r.
-           rewrite <- OpenNat.add_0_r at 1.
-           unfold lt.
-           rewrite <- OpenNat.add_succ_l.
-           apply OpenNat.add_le_mono.
-           ++ apply OpenNat.le_0_n.
-           ++ exact IHz.
-       }
-       exact (G n).
-Defined.
-
-Add Parametric Morphism
-    (n: nat)
-  : (box n)
-    with signature (eq) ==> (@mem_eq n)
-      as box_morph.
-Proof.
-  intros y.
-  reflexivity.
-Defined.
+  apply Nat.mod_upper_bound.
+  apply Nat.pow_nonzero.
+  intro H; discriminate.
+Qed.
 
 Definition zero
            (n: nat)
@@ -163,16 +159,13 @@ Definition unbox
   mem_val x.
 
 Add Parametric Morphism
-    (n: nat)
-  : (@unbox n)
-    with signature (@mem_eq n) ==> eq
+    (n:  nat)
+  : (@unbox n) with signature (@mem_eq n) ==> eq
       as unbox_morphism.
-Proof.
-  intros x y H.
+  intros x y [Heq].
   unfold unbox.
-  rewrite H.
-  reflexivity.
-Defined.
+  exact Heq.
+Qed.
 
 Definition cast
            {n: nat}
@@ -188,8 +181,9 @@ Add Parametric Morphism
     with signature (@mem_eq n) ==> eq
       as cast_morphism.
 Proof.
-  intros x y H.
+  intros x y [H].
   unfold cast.
+  unfold unbox.
   rewrite H.
   reflexivity.
 Defined.
@@ -201,17 +195,29 @@ Lemma cast_same_size_eq
 Proof.
   unfold cast.
   unfold box.
-  unfold mem_eq.
+  unfold unbox.
+  constructor.
+  destruct x as [x Hbound].
   cbn.
-  destruct lt_dec.
-  + unfold unbox.
-    reflexivity.
-  + assert (unbox x < 2 ^ n). {
-      unfold unbox.
-      apply (mem_bound x).
-    }
-    apply n0 in H.
-    destruct H.
+  apply Nat.mod_small.
+  exact Hbound.
+Qed.
+
+Lemma cast_cast_is_cast
+      {n m:  nat}
+      (x:    mem n)
+  : mem_eq (cast m (cast m x)) (cast m x).
+Proof.
+  unfold cast.
+  unfold unbox.
+  unfold box.
+  destruct x.
+  unfold mem_val.
+  constructor.
+  unfold mem_val.
+  rewrite Nat.mod_mod; [ reflexivity |].
+  apply Nat.pow_nonzero.
+  intro H; discriminate.
 Qed.
 
 (** ** Arithmetic
@@ -304,60 +310,6 @@ Definition mltb
   : bool :=
   unbox x <? unbox y.
 
-(** * Memory
-
- *)
-
-Inductive Endianness : Type := BE | LE.
-
-Local Open Scope list_scope.
-
-Fixpoint split
-         (n: nat)
-         (x: mem (8 * n))
-         {struct n}
-  : list byte :=
-  match n with
-  | 0 => []
-  | S m => (cast 8 x)::(split m (cast (8 * m) (shiftr x 8)))
-  end.
-
-Program Definition split_word
-        (x: word)
-  : byte * byte :=
-  match split 2 x with
-  | b1 :: b2 :: nil => (b1, b2)
-  | _ => !
-  end.
-Next Obligation.
-  assert ([cast 8 x; cast 8 (cast 8 (shiftr x 8))] <> [cast 8 x; cast 8 (cast 8 (shiftr x 8))])
-    by apply H.
-  destruct H0.
-  reflexivity.
-Defined.
-
-Program Definition split_lword
-        (x: lword)
-  : byte * byte * byte * byte :=
-  match split 4 x with
-  | b1 :: b2 :: b3 :: b4 :: nil => (b1, b2, b3, b4)
-  | _ => !
-  end.
-Next Obligation.
-  assert (
-      [cast 8 x; cast 8 (cast 24 (shiftr x 8));
-      cast 8 (cast 16 (shiftr (cast 24 (shiftr x 8)) 8));
-      cast 8 (cast 8 (shiftr (cast 16 (shiftr (cast 24 (shiftr x 8)) 8)) 8))]
-        <>
-      [cast 8 x; cast 8 (cast 24 (shiftr x 8));
-      cast 8 (cast 16 (shiftr (cast 24 (shiftr x 8)) 8));
-      cast 8 (cast 8 (shiftr (cast 16 (shiftr (cast 24 (shiftr x 8)) 8)) 8))]
-    )
-    by apply H.
-  destruct H0.
-  reflexivity.
-Defined.
-
 (** * Manipulation
 
   *)
@@ -369,3 +321,242 @@ Definition append
   : mem (n + m) :=
   add (shiftl (cast (n + m) v') n)
       (cast (n + m) v).
+
+Add Parametric Morphism
+    (n m:  nat)
+  : (@append n m) with signature mem_eq ==> mem_eq ==> mem_eq
+      as append_morphism.
+  intros x x' [Heq] y y' [Heq'].
+  constructor.
+  unfold append.
+  unfold cast.
+  unfold shiftl, add.
+  unfold unbox, box.
+  unfold mem_val.
+  destruct   x   as [x  Hx];
+    destruct x'  as [x' Hx'];
+    destruct y   as [y  Hy];
+    destruct y'  as [y' Hy'].
+  cbn in *.
+  subst.
+  reflexivity.
+Qed.
+
+(** * Memory
+
+ *)
+
+Definition upper_half
+           (n:  nat)
+           (x:  mem (2 * n))
+  : mem n :=
+  cast n (shiftr x n).
+
+Definition lower_half
+           (n:  nat)
+           (x:  mem (2 * n))
+  : mem n :=
+  cast n x.
+
+Definition join
+           (n:    nat)
+           (h l:  mem n)
+  : mem (2 * n) :=
+  add (cast (2 * n) l) (shiftl (cast (2 * n) h) n).
+
+Lemma pow_pos
+      (a b:  nat)
+  : 0 < a -> 0 < a ^ b.
+Proof.
+  intros H.
+  apply neq_0_lt.
+  apply Nat.neq_sym.
+  eapply Nat.pow_nonzero.
+  apply lt_0_neq in H.
+  apply Nat.neq_sym.
+  exact H.
+Qed.
+
+Lemma shiftr_reduces
+      {n m:  nat}
+  : Nat.shiftr n m <= n.
+Proof.
+  revert n.
+  induction m.
+  + cbn.
+    reflexivity.
+  + intros n.
+    cbn.
+    apply Nat.div2_decr.
+    transitivity n.
+    ++ apply IHm.
+    ++ constructor.
+       reflexivity.
+Qed.
+
+Lemma div2_prop
+      (x r:  nat)
+      (H:    x < 2 ^ r)
+  : Nat.div2 x < 2 ^ Nat.pred r.
+Proof.
+  apply <- (Nat.mul_lt_mono_pos_l 2); [| omega ].
+  apply (Nat.le_lt_trans (2 * Nat.div2 x) x).
+  + transitivity (2 * Nat.div2 x + Nat.b2n (Nat.odd x)).
+    ++ omega.
+    ++ rewrite <- (Nat.div2_odd x).
+       reflexivity.
+  + induction r.
+    ++ cbn in *.
+       omega.
+    ++ cbn.
+       rewrite add_0_r.
+       assert (Heq:  2 ^ r + 2 ^ r = 2 * (2 ^ r)) by omega.
+       rewrite Heq.
+       rewrite <- Nat.pow_succ_r.
+       exact H.
+       omega.
+Qed.
+
+Lemma shiftr_reduces'
+      {x n m: nat}
+      (H: x < 2 ^ n)
+  : Nat.shiftr x m < 2 ^ (n - m).
+Proof.
+  revert x n H.
+  induction m.
+  + cbn.
+    intros x n H.
+    rewrite sub_0_r.
+    exact H.
+  + intros x n H.
+    cbn.
+    remember (Nat.shiftr x m) as x'.
+    cbn in x'.
+    assert (H':  Nat.shiftr x m < 2 ^ (n - m)). {
+      apply IHm.
+      exact H.
+    }
+    rewrite <- Heqx' in H'.
+    rewrite Nat.sub_succ_r.
+    remember (n - m) as r.
+    apply div2_prop.
+    exact H'.
+Qed.
+
+Lemma shiftl_shiftr_div
+      (x n:  nat)
+  : Nat.shiftl (Nat.shiftr x n) n = (2 ^ n) * (x / (2 ^ n)).
+Proof.
+  rewrite Nat.shiftr_div_pow2.
+  rewrite Nat.shiftl_mul_pow2.
+  apply Nat.mul_comm.
+Qed.
+
+Lemma shiftr_shiftl_le
+      (x n:  nat)
+  : Nat.shiftl (Nat.shiftr x n) n <= x.
+Proof.
+  rewrite shiftl_shiftr_div.
+  remember (2 ^ n) as r.
+  apply Nat.mul_div_le.
+  induction n.
+  + cbn in Heqr.
+    rewrite Heqr.
+    auto.
+  + rewrite Heqr.
+    apply Nat.neq_sym.
+    apply lt_0_neq.
+    apply pow_pos.
+    repeat constructor.
+Qed.
+
+Lemma split_merge_eq
+      (n: nat)
+      (x: mem (2 * n))
+  : mem_eq x (join n (upper_half n x) (lower_half n x)).
+Proof.
+  constructor.
+  destruct x as [x Hx].
+  unfold join, lower_half, upper_half, shiftl, shiftr, add, cast, box, unbox.
+  unfold mem_val.
+  rewrite (Nat.mod_small (x mod 2 ^ n) (2 ^ (2 * n))).
+  + rewrite (Nat.mod_small ((Nat.shiftr x n mod 2 ^ (2 * n)) mod 2 ^ n) (2 ^ (2 * n))).
+    ++ rewrite (Nat.mod_small (Nat.shiftr x n) (2 ^ (2 * n))).
+       +++ rewrite (Nat.mod_small (Nat.shiftr x n) (2 ^ n)).
+           ++++ rewrite (Nat.mod_small (Nat.shiftl (Nat.shiftr x n) n) (2 ^ (2 * n))); [| apply (Nat.le_lt_trans _ x); [| exact Hx ];
+                                                                                          apply shiftr_shiftl_le
+                                                                                       ].
+                rewrite shiftl_shiftr_div.
+                rewrite Nat.add_comm.
+                rewrite <- Nat.div_mod.
+                rewrite (Nat.mod_small _ _ Hx).
+                reflexivity.
+                apply Nat.neq_sym.
+                apply lt_0_neq.
+                apply pow_pos.
+                omega.
+           ++++ assert (Hhelper:  forall (a:  nat), 2 * a - a = a). {
+                  clear Hx x n.
+                  induction a.
+                  + reflexivity.
+                  + cbn.
+                    rewrite add_0_r.
+                    rewrite (Nat.add_comm a (S a)).
+                    rewrite <- Nat.add_sub_assoc.
+                    ++ rewrite Nat.sub_diag.
+                       rewrite add_0_r.
+                       reflexivity.
+                    ++ constructor.
+                }
+                rewrite <- (Hhelper n) at 2.
+                apply shiftr_reduces'.
+                exact Hx.
+       +++ apply (Nat.le_lt_trans _ x); [| exact Hx ].
+           apply shiftr_reduces.
+    ++ apply (Nat.lt_le_trans _ (2 ^ n)).
+       +++ apply Nat.mod_bound_pos.
+           apply le_0_n.
+           apply pow_pos.
+           auto.
+       +++ apply Nat.pow_le_mono_r; omega.
+  + apply (Nat.lt_le_trans (x mod (2 ^ n)) (2 ^ n)).
+    ++ apply Nat.mod_bound_pos.
+       apply le_0_n.
+       apply pow_pos.
+       auto.
+    ++ apply Nat.pow_le_mono_r; omega.
+Qed.
+
+Program Definition split_word
+        (x: word)
+  : byte * byte :=
+  (upper_half 8 x, lower_half 8 x).
+
+Program Definition split_lword
+        (x: lword)
+  : byte * byte * byte * byte :=
+  (fst (split_word (upper_half 16 x)),
+   snd (split_word (upper_half 16 x)),
+   fst (split_word (lower_half 16 x)),
+   snd (split_word (lower_half 16 x))
+   ).
+
+Definition qfst
+           {A B C D:  Type}
+  : A * B * C * D -> A :=
+  fst <<< fst <<< fst.
+
+Definition qsnd
+           {A B C D:  Type}
+  : A * B * C * D -> B :=
+  snd <<< fst <<< fst.
+
+Definition qthrd
+           {A B C D:  Type}
+  : A * B * C * D -> C :=
+  snd <<< fst.
+
+Definition qlst
+           {A B C D:  Type}
+  : A * B * C * D -> D :=
+  snd.
